restoring PRFSetHash

steel/Veritas.Steel.PRFSetHash.fst
@@ -19,16 +19,16 @@ module VF = Veritas.Formats
 module MSH = Veritas.MultiSetHash
 module HA = Veritas.Steel.HashAccumulator
 #push-options "--query_stats"
-#push-options "--fuel 2 --ifuel 1" //not sure why some proofs need fuel 2
+#push-options "--fuel 2 --ifuel 1" // some proofs need fuel 2; because of needing to unroll t_of
 noeq
 type prf_set_hash = {
-  ha_state : HA.state;
+  ha_state : HA.ha;
   serialization_buf: a:A.array U8.t{A.length a == 184 }
 }
 
 let prf_set_hash_vprop (s:prf_set_hash)
   : vprop
-  = A.varray s.ha_state `star`
+  = HA.ha_inv s.ha_state `star`
     A.varray s.serialization_buf
 
 let prf_set_hash_sl (s:prf_set_hash)
@@ -37,9 +37,9 @@ let prf_set_hash_sl (s:prf_set_hash)
 
 let prf_set_hash_repr
   : Type0
-  = (HA.hash_value_t & A.contents U8.t 184)
+  = (HA.ha_repr & A.contents U8.t 184)
 
-let hash_value_of (p:prf_set_hash_repr) = fst p
+let hash_value_of (p:prf_set_hash_repr) = HA.value_of (fst p)
 
 let prf_set_hash_sel (r:prf_set_hash)
   : GTot (selector prf_set_hash_repr (prf_set_hash_sl r))
@@ -47,12 +47,12 @@ let prf_set_hash_sel (r:prf_set_hash)
 
 let intro_set_hash_inv #o (s:prf_set_hash)
   : SteelGhost unit o
-    (A.varray s.ha_state `star` A.varray s.serialization_buf)
+    (HA.ha_inv s.ha_state `star` A.varray s.serialization_buf)
     (fun _ -> prf_set_hash_inv s)
     (requires fun _ -> True)
     (ensures fun h0 _ h1 ->
-      v_hash s h1 == A.asel s.ha_state h0)
-  = AT.change_slprop_rel (A.varray s.ha_state `star` A.varray s.serialization_buf)
+      v_hash s h1 == HA.hash_value_of s.ha_state h0)
+  = AT.change_slprop_rel (HA.ha_inv s.ha_state `star` A.varray s.serialization_buf)
                          (prf_set_hash_inv s)
                          (fun x y -> x == y)
                          (fun m -> ())
@@ -60,98 +60,66 @@ let intro_set_hash_inv #o (s:prf_set_hash)
 let elim_set_hash_inv #o (s:prf_set_hash)
   : SteelGhost unit o
     (prf_set_hash_inv s)
-    (fun _ -> A.varray s.ha_state `star` A.varray s.serialization_buf)
+    (fun _ -> HA.ha_inv s.ha_state `star` A.varray s.serialization_buf)
     (requires fun _ -> True)
     (ensures fun h0 _ h1 ->
-      v_hash s h0 == A.asel s.ha_state h1)
+      v_hash s h0 == HA.hash_value_of s.ha_state h1)
   = AT.change_slprop_rel (prf_set_hash_inv s)
-                         (A.varray s.ha_state `star` A.varray s.serialization_buf)
+                         (HA.ha_inv s.ha_state `star` A.varray s.serialization_buf)
                          (fun x y -> x == y)
                          (fun m -> ())
 
-let create () =
-  let x = HA.create_in () in
+let create x =
   let buf = A.malloc 0uy 184ul in
   let res = {
     ha_state = x;
     serialization_buf = buf
   } in
-  AT.change_equal_slprop (A.varray x `star` A.varray buf)
-                         (A.varray res.ha_state `star` A.varray res.serialization_buf);
+  AT.change_equal_slprop (HA.ha_inv x `star` A.varray buf)
+                         (HA.ha_inv res.ha_state `star` A.varray res.serialization_buf);
   intro_set_hash_inv res;
   AT.return res
 
 let free (p:prf_set_hash)
   = elim_set_hash_inv p;
-    HA.free p.ha_state;
-    A.free p.serialization_buf
+    A.free p.serialization_buf;
+    AT.return p.ha_state
 
-//#push-options "--query_stats"
-let prf_update_hash' (p:HA.state)
+let prf_update_hash' (p:HA.ha)
                      (r:T.record)
                      (t:T.timestamp)
                      (tid:T.thread_id)
                      (buf:A.array U8.t)
-  : Steel unit
-    (A.varray p `star` A.varray buf)
-    (fun _ -> A.varray p `star` A.varray buf)
+  : Steel bool
+    (HA.ha_inv p `star` A.varray buf)
+    (fun _ -> HA.ha_inv p `star` A.varray buf)
     (requires fun _ ->
-      A.length p == 32 /\
       A.length buf == 184)
-    (ensures fun h0 _ h1 ->
-      A.asel p h1 == VM.update_hash_value (A.asel p h0) r t tid)
+    (ensures fun h0 b h1 ->
+      HA.hash_value_of p h1 ==
+      maybe_update_hash_value b (HA.hash_value_of p h0) r t tid)
   =  let h0 = AT.get () in
      let sr = (VFT.({ sr_record = r; sr_timestamp = t; sr_thread_id = tid})) in
      let len = VF.serialize_stamped_record buf sr in
      let h1 = AT.get () in
-     HA.add p buf len;
-     AT.slassert (A.varray p);
+     let b = HA.add p buf len in
      let h2 = AT.get () in
-     assert (A.asel p h2 ==
-             HA.aggregate_hash_value (A.asel p h1)
-                                     (HA.hash_value
-                                       (Seq.slice (A.asel buf h1) 0 (U32.v len))));
+     assert (HA.hash_value_of p h2 ==
+             HA.maybe_aggregate_hashes
+                 b
+                 (HA.hash_value_of p h1)
+                 (HA.hash_one_value
+                   (Seq.slice (A.asel buf h1) 0 (U32.v len))));
      assert (Seq.slice (A.asel buf h1) 0 (U32.v len) ==
              VF.serialize_stamped_record_spec sr);
-     assert (A.asel p h2 ==
-             HA.aggregate_hash_value
-               (A.asel p h1)
-               (HA.hash_value (VF.serialize_stamped_record_spec sr)));
-     assert_spinoff (A.asel p h2 ==
-                     VM.update_hash_value (A.asel p h1) r t tid)
+     assert (HA.hash_value_of p h2 ==
+             HA.maybe_aggregate_hashes b
+               (HA.hash_value_of p h1)
+               (HA.hash_one_value (VF.serialize_stamped_record_spec sr)));
+     AT.return b
 
 let prf_update_hash p r t tid =
   elim_set_hash_inv p;
-  prf_update_hash' p.ha_state r t tid p.serialization_buf;
-  intro_set_hash_inv p
-
-let prf_read_hash' (p:HA.state) (out:A.array U8.t)
-  : Steel unit
-    (A.varray p `star` A.varray out)
-    (fun _ -> A.varray p `star` A.varray out)
-    (requires fun _ -> A.length out == 32)
-    (ensures fun h0 _ h1 ->
-      A.length out == 32 /\
-      A.asel p h0 == A.asel p h1 /\
-      A.asel out h1 == A.asel p h1)
-  = HA.get p out
-
-let prf_read_hash (p:prf_set_hash) (out:A.array U8.t)
-  = elim_set_hash_inv p;
-    prf_read_hash' p.ha_state out;
-    intro_set_hash_inv p
-
-let prf_hash_agg (a0 a1:A.array U8.t)
-  : Steel unit
-    (A.varray a0 `star` A.varray a1)
-    (fun _ -> A.varray a0 `star` A.varray a1)
-    (requires fun _ ->
-      A.length a0 == 32 /\
-      A.length a1 == 32)
-    (ensures fun h0 _ h1 ->
-      A.length a0 == 32 /\
-      A.length a1 == 32 /\
-      A.asel a1 h0 == A.asel a1 h1 /\
-      A.asel a0 h1 ==
-        HA.aggregate_hash_value (A.asel a0 h0) (A.asel a1 h0))
-  = HA.aggregate_hash_value_buf a0 a1
+  let b = prf_update_hash' p.ha_state r t tid p.serialization_buf in
+  intro_set_hash_inv p;
+  AT.return b
