steel/Veritas.Steel.PRFSetHash.fsti
@@ -56,9 +56,10 @@ let v_hash (#p:vprop)
 
 val create (ha:HA.ha)
   : Steel prf_set_hash
-    emp
+    (HA.ha_inv ha)
     (fun p -> prf_set_hash_inv p)
-    (requires fun _ -> True)
+    (requires fun h0 ->
+       HA.hash_value_of ha h0 == HA.initial_hash)
     (ensures fun _ p h1 -> v_hash p h1 == HA.initial_hash)
 
 val free (p:prf_set_hash)
@@ -70,37 +71,24 @@ val free (p:prf_set_hash)
       v_hash p h0 ==
       HA.hash_value_of x h1)
 
+let maybe_update_hash_value (b:bool)
+                            (ha:HA.hash_value_t)
+                            (r:T.record)
+                            (t:T.timestamp)
+                            (tid:T.thread_id)
+  : GTot HA.hash_value_t
+  = if b
+    then VM.update_hash_value ha r t tid
+    else ha
+
 val prf_update_hash (p:prf_set_hash)
                     (r:T.record)
                     (t:T.timestamp)
                     (thread_id:T.thread_id)
-  : Steel unit
+  : Steel bool
     (prf_set_hash_inv p)
     (fun _ -> prf_set_hash_inv p)
     (requires fun _ -> True)
-    (ensures fun h0 _ h1 ->
-      v_hash p h1 == VM.update_hash_value (v_hash p h0) r t thread_id)
-
-// val prf_read_hash (p:prf_set_hash) (out:A.array U8.t)
-//   : Steel unit
-//     (prf_set_hash_inv p `star` A.varray out)
-//     (fun _ -> prf_set_hash_inv p `star` A.varray out)
-//     (requires fun _ -> A.length out == 32)
-//     (ensures fun h0 _ h1 ->
-//       A.length out == 32 /\
-//       v_hash p h0 == v_hash p h1 /\
-//       A.asel out h1 == v_hash p h1)
-
-// val prf_hash_agg (a0 a1:A.array U8.t)
-//   : Steel unit
-//     (A.varray a0 `star` A.varray a1)
-//     (fun _ -> A.varray a0 `star` A.varray a1)
-//     (requires fun _ ->
-//       A.length a0 == 32 /\
-//       A.length a1 == 32)
-//     (ensures fun h0 _ h1 ->
-//       A.length a0 == 32 /\
-//       A.length a1 == 32 /\
-//       A.asel a1 h0 == A.asel a1 h1 /\
-//       A.asel a0 h1 ==
-//         HA.aggregate_hashes (A.asel a0 h0) (A.asel a1 h0))
+    (ensures fun h0 b h1 ->
+      v_hash p h1 ==
+      maybe_update_hash_value b (v_hash p h0) r t thread_id)
